prove assignment

src/untyped.lean
@@ -40,9 +40,6 @@ inductive valid_int_expression : expression → ℕ → Prop
 | add {e₁ e₂ n₁ n₂} (h₁ : valid_int_expression e₁ n₁) (h₂ : valid_int_expression e₂ n₂) : valid_int_expression (add e₁ e₂) (n₁ + n₂)
 | literal {n} : valid_int_expression (literal_int n) n
 
--- def pred_on_list (α : Type) : list α → Prop
--- | (x :: xs) := 
-
 inductive program
 | assign (n : string) : list (expression) → expression → program
 | seq : program → program → program
@@ -52,10 +49,18 @@ inductive program
 infixr ` ;; `:90 := program.seq
 open program
 
+def pred_on_list {α : Type} (f : α → Prop) : list α → Prop
+| (x :: xs) := f x ∧ pred_on_list xs
+| [] := true
+
+@[reducible]
+def int_expression_list_eval (idx_expr : list expression) (idx_evaled : list ℕ) := 
+    pred_on_list (λ x : (expression × ℕ), valid_int_expression x.1 x.2) (idx_expr.zip idx_evaled) ∧
+    idx_expr.length = idx_evaled.length
+
 inductive big_step : (program × state) → state → Prop
 | assign_global_int {n expr val} {s u : state} {idx_expr : list expression} {idx_evaled : list ℕ} (h_eval : valid_int_expression expr val) 
-    -- (h_idx : (idx_expr.zip idx_evaled).all (λ x, valid_int_expression x.1 x.2))
-    (h_idx_length : idx_expr.length = idx_evaled.length)
+    (h_idx : int_expression_list_eval idx_expr idx_evaled)
     (h_carryover : ∀ m m_idx, ¬(n = m ∧ idx_evaled = m_idx) → u.global m m_idx = s.global m m_idx)
     (h_updated : u.global n idx_evaled = val) : 
     big_step ((assign n idx_expr expr), s) u
@@ -64,23 +69,132 @@ inductive big_step : (program × state) → state → Prop
 
 infix ` ⟹ `:110 := big_step
 
-def p : program :=
-    assign "n" [] (literal_int 0)
+lemma pred_on_list_head {α : Type} {xs : list α} {f x} (hp : pred_on_list f (x :: xs)) : f x := begin
+    rw pred_on_list at hp,
+    cases hp, 
+    assumption,
+end
 
-theorem x : {string_imp . data := ['n']} = "n" := by refl
+lemma pred_on_list_tail {α : Type} {xs : list α} {f x} (hp : pred_on_list f (x :: xs)) : pred_on_list f xs := begin
+    rw pred_on_list at hp,
+    cases hp, 
+    assumption,
+end
 
-example {s u} (hp : (p, s) ⟹ u) : u.global "n" [] = 1 := begin
-    cases hp,
-    simp * at *,
-    have : hp_idx_evaled = [] := begin
+lemma list_length_neq_zero {α} {l : list α} (h : ¬(l.length = 0)) : ∃ x xs, l = (x :: xs) := begin
+    cases l,
+    case list.nil {
+        simp at h,
+        contradiction
+    },
+    case list.cons {
+        apply Exists.intro l_hd,
+        apply Exists.intro l_tl,
+        refl,
+    }
+end
+
+lemma list_length_tail {α β : Type} {x : α} {y : β} {xs ys} (h : (x :: xs).length = (y :: ys).length) : xs.length = ys.length := begin
+    rw list.length at h,
+    rw list.length at h,
+    simp at h,
+    repeat { rw nat.one_add at h },
+    simp at h,
+    assumption,
+end
+
+lemma valid_int_expression_eq {expr r₁ r₂} (h₁ : valid_int_expression expr r₁) (h₂ : valid_int_expression expr r₂) : r₁ = r₂ := begin
+    cases h₁;
+        cases h₂;
+        try {refl},
+    sorry
+end
+
+theorem int_expression_list_unique {expr eval₁ eval₂} (h₁ : int_expression_list_eval expr eval₁) (h₂ : int_expression_list_eval expr eval₂) : eval₁ = eval₂ := begin
+    cases h₁,
+    cases h₂,
+    induction eval₁ generalizing eval₂ expr, -- can pick any list (generalizing the others)
+    case list.nil {
+        rw h₁_right at h₂_right,
+        simp at h₂_right,
+        apply eq.symm,
         apply list.eq_nil_of_length_eq_zero,
         apply eq.symm,
-        assumption
+        assumption,
+    },
+    case list.cons {
+        -- break out head form eval₂
+        have : ∃ x xs, eval₂ = (x :: xs) := begin
+            apply list_length_neq_zero,
+            rw ← h₂_right,
+            rw h₁_right,
+            trivial,
+        end,
+        cases this with eval₂_hd,
+        cases this_h with eval₂_tl eval₂_eq,
+        subst eval₂_eq,
+        -- break out head from expr
+        have : ∃ x xs, expr = (x :: xs) := begin
+            apply list_length_neq_zero,
+            rw h₁_right,
+            trivial,
+        end,
+        cases this with expr_hd,
+        cases this_h with expr_tl expr_eq,
+        subst expr_eq,
+        have : eval₁_hd = eval₂_hd := begin
+            have : valid_int_expression expr_hd eval₁_hd := begin
+                rw list.zip at h₁_left,
+                rw list.zip_with at h₁_left,
+                apply pred_on_list_head h₁_left,
+            end,
+            have : valid_int_expression expr_hd eval₂_hd := begin
+                rw list.zip at h₂_left,
+                rw list.zip_with at h₂_left,
+                apply pred_on_list_head h₂_left,
+            end,
+            apply valid_int_expression_eq,
+            repeat { assumption },
+        end,
+        cases this,
+        have : eval₁_tl = eval₂_tl := begin
+            apply (@eval₁_ih eval₂_tl expr_tl),
+            {
+                apply pred_on_list_tail h₁_left,
+            }, {
+                apply list_length_tail h₁_right,
+            }, {
+                apply pred_on_list_tail h₂_left,
+            }, {
+                apply list_length_tail h₂_right,
+            }
+        end,
+        cases this,
+        refl,
+    }
+end
+
+@[simp]
+lemma big_step_assign {s u val n idx_expr idx_evaled} (hp : ((assign n idx_expr (literal_int val)), s) ⟹ u) (hi : int_expression_list_eval idx_expr idx_evaled) : 
+    u.global n idx_evaled = val := 
+begin
+    cases hp,
+    have : hp_idx_evaled = idx_evaled := begin
+        apply int_expression_list_unique hp_h_idx hi,
     end,
     rw <- this,
-    rw x at hp_h_updated,
     rw hp_h_updated,
     cases hp_h_eval,
+    refl,
+end
+
+def p : program :=
+    assign "n" [] (literal_int 1)
+
+example {s u} (hp : (p, s) ⟹ u) : u.global "n" [] = 1 := begin
+    apply big_step_assign,
+    assumption,
+    
 end
 
 end MCL_untyped
